Add more syntax

example.v
@@ -9,51 +9,49 @@ Open Scope string_scope.
 Open Scope Z_scope.
 
 Example ex1 :=
-  <{ let "f" =
-         reset begin
-           let "x" = 6 * 9 in
-           let "y" = (shift "k" => "k") in
-           "x" * "y"
-         end
+  <{ let "f" :=
+       reset
+         let "x" := 6 * 9 in
+         let "y" := shift "k" "k" in
+         "x" * "y"
      in
      "f" 10 }>.
 
 Compute (eval_term 2 ex1).
 
 Example append_aux :=
-  <{ fix "append_aux" "xs" =>
+  <{ fix "append_aux" "xs" :=
        match "xs" with
-       | Inl {BAnon} => shift "k" => "k"
+       | Inl _ => shift "k" "k"
        | Inr "xs" =>
-           let "x", "xs'" = "xs" in
-           let "r" = "append_aux" "xs'" in
-           let "r" = "x", "r" in
+           let ("x", "xs'") := "xs" in
+           let "r" := "append_aux" "xs'" in
+           let "r" := ("x", "r") in
            Inr "r"
        end }>.
 
 Example append :=
-  <{ let "append_aux" = {append_aux} in
+  <{ let "append_aux" := append_aux in
      fun "xs" => reset "append_aux" "xs" }>.
 
 Fixpoint encode (xs : list Z) :=
   match xs with
   | [] => <{ Inl () }>
-  | x :: xs' =>
-      <{ let "xs'" = {encode xs'} in
-         let "xs" = {x}, "xs'" in
-         Inr "xs" }>
+  | x :: xs' => <{ let "xs'" := {encode xs'} in
+                   let "xs" := (x, "xs'") in
+                   Inr "xs" }>
   end.
 
 Example append1 xs :=
-  <{ let "append" = {append} in
-     let "xs" = {xs} in
+  <{ let "append" := append in
+     let "xs" := xs in
      "append" "xs" }>.
 
 Example append2 xs ys :=
-  <{ let "append" = {append} in
-     let "xs" = {xs} in
-     let "ys" = {ys} in
-     let "append1" = "append" "xs" in
+  <{ let "append" := append in
+     let "xs" := xs in
+     let "ys" := ys in
+     let "append1" := "append" "xs" in
      "append1" "ys" }>.
 
 Compute (eval_term 3 (append1 (encode []))).
@@ -64,31 +62,31 @@ Compute (eval_term 4 (append2 (encode [1]) (encode [2]))).
 Fixpoint sequence start len : list Z :=
   match len with
   | O => []
-  | S len' => start :: sequence (Z.succ start) len'
+  | S len' => start :: sequence (start + 1) len'
   end.
 
 Example append_direct :=
-  <{ fix "append_direct" "xs" "ys" =>
+  <{ fix "append_direct" "xs" "ys" :=
        match "xs" with
-       | Inl {BAnon} => "ys"
+       | Inl _ => "ys"
        | Inr "xs" =>
-           let "x", "xs'" = "xs" in
-           let "append_direct1" = "append_direct" "xs'" in
-           let "r" = "append_direct1" "ys" in
-           let "r" = "x", "r" in
+           let ("x", "xs'") := "xs" in
+           let "append_direct1" := "append_direct" "xs'" in
+           let "r" := "append_direct1" "ys" in
+           let "r" := ("x", "r") in
            Inr "r"
        end }>.
 
 Example append_direct1 xs :=
-  <{ let "append_direct" = {append_direct} in
-     let "xs" = {xs} in
+  <{ let "append_direct" := append_direct in
+     let "xs" := xs in
      "append_direct" "xs" }>.
 
 Example append_direct2 xs ys :=
-  <{ let "append_direct" = {append_direct} in
-     let "xs" = {xs} in
-     let "ys" = {ys} in
-     let "append_direct1" = "append_direct" "xs" in
+  <{ let "append_direct" := append_direct in
+     let "xs" := xs in
+     let "ys" := ys in
+     let "append_direct1" := "append_direct" "xs" in
      "append_direct1" "ys" }>.
 
 Compute (eval_term 2 (append_direct1 (encode []))).
@@ -98,3 +96,57 @@ Compute (eval_term 3 (append_direct2 (encode [1]) (encode [2]))).
 
 Time Compute (eval_term 2000 (encode (sequence 0 1000))).
 Time Compute (eval_term_kont 2000 (encode (sequence 0 1000)) KNil).
+
+Example either :=
+  <{ fun "x" "y" => shift "k" let _ := "k" "x" in "k" "y" }>.
+
+Example ex2 :=
+  <{ let "either" := either in
+     let "result" := ref false in
+     let _ :=
+       reset
+         let "either1" := "either" true in
+         let "p" := "either1" false in
+         let "q" := "either1" false in
+         let "not_p" := not "p" in
+         let "not_q" := not "q" in
+         let "c1" := "p" || "q" in
+         let "c2" := "p" || "not_q" in
+         let "c3" := "not_p" || "not_q" in
+         let "r" := "c1" && "c2" in
+         let "r" := "r" && "c3" in
+         if "r" then "result" <- true else ()
+     in !"result" }>.
+
+Compute (eval_term 6 ex2).
+
+Example choice :=
+  <{ fun "xs" =>
+       shift "k"
+         let fix "go" "xs" :=
+           match "xs" with
+           | Inl _ => ()
+           | Inr "xs" =>
+               let ("x", "xs'") := "xs" in
+               let _ := "k" "x" in
+               "go" "xs'"
+           end
+         in "go" "xs" }>.
+
+Example sum xs :=
+  <{ let "choice" := choice in
+     let "xs" := xs in
+     let "result" := ref 0 in
+     let _ :=
+       reset
+         let "x" := "choice" "xs" in
+         let "r" := !"result" in
+         let "r" := "r" + "x" in
+         "result" <- "r"
+     in !"result" }>.
+
+Compute (run_term 3 (sum (encode []))).
+Compute (run_term 4 (sum (encode [1]))).
+Compute (run_term 5 (sum (encode [1; 2]))).
+
+Time Compute (run_term 1000 (sum (encode (sequence 0 500)))).
