shift-reset/core/syntax_notation.v
@@ -9,9 +9,8 @@ Declare Custom Entry term.
 
 Notation "<{ t }>" := t (t custom term at level 99) : term_scope.
 Notation "( t )" := t (in custom term, t at level 99) : term_scope.
-Notation "{ t }" := t (in custom term, t constr) : term_scope.
 Notation "t" := t (in custom term at level 0, t constr at level 0) : term_scope.
-Notation "'begin' t 'end'" := t (in custom term, t custom term at level 99, only parsing) : term_scope.
+Notation "{ t }" := t (in custom term, t constr) : term_scope.
 
 Notation "a1 a2" :=
   (TApp a1 a2)
@@ -26,7 +25,7 @@ Notation "'if' a 'then' t1 'else' t2" :=
         t1 custom term,
         t2 custom term) : term_scope.
 
-Notation "'let' x '=' t1 'in' t2" :=
+Notation "'let' x := t1 'in' t2" :=
   (TLet t1 (T1 x t2))
     (in custom term at level 69,
         x at level 0,
@@ -34,7 +33,7 @@ Notation "'let' x '=' t1 'in' t2" :=
         t2 custom term,
         right associativity) : term_scope.
 
-Notation "'let' f x1 .. xn '=' t1 'in' t2" :=
+Notation "'let' f x1 .. xn := t1 'in' t2" :=
   (TLet (TFun (T1 x1 .. (TFun (T1 xn t1)) ..)) (T1 f t2))
     (in custom term at level 69,
         f, x1, xn at level 0,
@@ -42,7 +41,7 @@ Notation "'let' f x1 .. xn '=' t1 'in' t2" :=
         t2 custom term,
         right associativity) : term_scope.
 
-Notation "'let' 'rec' f x '=' t1 'in' t2" :=
+Notation "'let' 'fix' f x := t1 'in' t2" :=
   (TLet (TFix (T2 f x t1)) (T1 f t2))
     (in custom term at level 69,
         f, x at level 0,
@@ -50,7 +49,7 @@ Notation "'let' 'rec' f x '=' t1 'in' t2" :=
         t2 custom term,
         right associativity) : term_scope.
 
-Notation "'let' 'rec' f x1 x2 .. xn '=' t1 'in' t2" :=
+Notation "'let' 'fix' f x1 x2 .. xn := t1 'in' t2" :=
   (TLet (TFix (T2 f x1 (TFun (T1 x2 .. (TFun (T1 xn t1)) ..)))) (T1 f t2))
     (in custom term at level 69,
         f, x1, x2, xn at level 0,
@@ -58,7 +57,7 @@ Notation "'let' 'rec' f x1 x2 .. xn '=' t1 'in' t2" :=
         t2 custom term,
         right associativity) : term_scope.
 
-Notation "'shift' k '=>' t" :=
+Notation "'shift' k t" :=
   (TShift (T1 k t))
     (in custom term at level 69,
         k at level 0,
@@ -67,25 +66,26 @@ Notation "'shift' k '=>' t" :=
 Notation "'reset' t" :=
   (TReset t) (in custom term at level 69, t custom term) : term_scope.
 
-Notation "'fun' x1 .. xn '=>' t" :=
+Notation "'fun' x1 .. xn => t" :=
   (TFun (T1 x1 .. (TFun (T1 xn t)) ..))
     (in custom term at level 69,
         x1, xn at level 0,
         t custom term at level 99) : term_scope.
 
-Notation "'fix' f x '=>' t" :=
+Notation "'fix' f x := t" :=
   (TFix (T2 f x t))
     (in custom term at level 69,
         f, x at level 0,
         t custom term at level 99) : term_scope.
 
-Notation "'fix' f x1 x2 .. xn '=>' t" :=
+Notation "'fix' f x1 x2 .. xn := t" :=
   (TFix (T2 f x1 (TFun (T1 x2 .. (TFun (T1 xn t)) ..))))
     (in custom term at level 69,
         f, x1, x2, xn at level 0,
         t custom term at level 99) : term_scope.
 
 Notation "()" := AUnit (in custom term at level 0) : term_scope.
+Notation "'_'" := BAnon (in custom term at level 0) : term_scope.
 
 Notation "'not' a" :=
   (TPrim1 P1Not a) (in custom term at level 23, a custom term at level 0) : term_scope.
@@ -123,13 +123,37 @@ Notation "a1 = a2" :=
         a1 custom term,
         a2 custom term) : term_scope.
 
+Notation "a1 <> a2" :=
+  (TPrim2 P2Eq a1 a2)
+    (in custom term at level 50,
+        a1 custom term,
+        a2 custom term) : term_scope.
+
 Notation "a1 < a2" :=
   (TPrim2 P2Lt a1 a2)
     (in custom term at level 50,
         a1 custom term,
         a2 custom term) : term_scope.
 
-Notation "a1 := a2" :=
+Notation "a1 && a2" :=
+  (TPrim2 P2And a1 a2)
+    (in custom term at level 50,
+        a1 custom term,
+        a2 custom term) : term_scope.
+
+Notation "a1 || a2" :=
+  (TPrim2 P2Or a1 a2)
+    (in custom term at level 50,
+        a1 custom term,
+        a2 custom term) : term_scope.
+
+Notation "a1 'xor' a2" :=
+  (TPrim2 P2And a1 a2)
+    (in custom term at level 50,
+        a1 custom term,
+        a2 custom term) : term_scope.
+
+Notation "a1 <- a2" :=
   (TSet a1 a2)
     (in custom term at level 65,
         a1 custom term,
@@ -141,7 +165,14 @@ Notation "a1 , a2" :=
         a1 custom term,
         a2 custom term) : term_scope.
 
-Notation "'let' x1 , x2 '=' a 'in' t" :=
+Notation "'let' ( x1 , x2 ) := a 'in' t" :=
+  (TSplit a (T2 x1 x2 t))
+    (in custom term at level 69,
+        x1, x2 at level 0,
+        t custom term,
+        right associativity) : term_scope.
+
+Notation "'let' x1 , x2 := a 'in' t" :=
   (TSplit a (T2 x1 x2 t))
     (in custom term at level 69,
         x1, x2 at level 0,
@@ -154,7 +185,7 @@ Notation "'Inl' a" :=
 Notation "'Inr' a" :=
   (TInr a) (in custom term at level 23, a custom term at level 0) : term_scope.
 
-Notation "'match' a 'with' '|' 'Inl' x1 '=>' t1 '|' 'Inr' x2 '=>' t2 'end'" :=
+Notation "'match' a 'with' | 'Inl' x1 => t1 | 'Inr' x2 => t2 'end'" :=
   (TCase a (T1 x1 t1) (T1 x2 t2))
     (in custom term at level 69,
         a custom term,
